semantics sets.lean
@@ -1,0 +1,533 @@
+import Std.Data.HashMap
+import Std.Data.HashSet
+import cvc5.Sql
+open Std
+
+def hashSet : HashSet Nat := HashSet.empty.insert 42 |>.insert 7
+
+#eval hashSet
+
+inductive DBValue
+ | boolValue (v: Option Bool)
+ | intValue (v: Option Int)
+ | stringValue (v: Option String)
+deriving BEq
+
+instance : Inhabited DBValue where
+  default := DBValue.boolValue false
+
+def less (a b : DBValue) : Bool :=
+  match a, b with
+  | .boolValue (some v1), .boolValue (some v2) => v1 ≤ v2
+  | .intValue (some v1), .intValue (some v2) => v1 ≤ v2
+  | .stringValue (some v1), .stringValue (some v2) => v1 ≤ v2
+  | _, _ => false
+
+def DBRow := List DBValue deriving BEq, Inhabited
+instance : Inhabited DBRow where
+  default := []
+
+instance : Hashable DBValue where
+  hash
+    | .boolValue (some v) => hash v
+    | .boolValue none => 0
+    | .intValue (some v) => hash v
+    | .intValue none => 0
+    | .stringValue (some v) => hash v
+    | .stringValue none => 0
+
+instance : Hashable DBRow where
+  hash row := row.foldl (fun acc x => mixHash acc (hash x)) 0
+
+def DBTable := HashMap DBRow Nat deriving Inhabited
+
+instance : Inhabited DBTable where
+  default := HashMap.empty
+
+instance : Hashable DBRow where
+  hash row := row.foldl (fun acc x => mixHash acc (hash x)) 0
+
+instance : Repr DBValue where
+  reprPrec v _ := match v with
+  | .boolValue v => s!"{v}"
+  | .intValue v => s!"{v}"
+  | .stringValue v => s!"{v}"
+
+def lessThan (a b : DBRow) : Bool :=
+ match a,b with
+ | [],[] => false
+ | a::as,b::bs => (less a b) && lessThan as bs
+ | [],_ => false
+ | _,[] => false
+
+
+namespace DBTable
+
+def mapRow (table: DBTable) (f: DBRow → DBRow) : DBTable :=
+  table.fold (fun acc x n => acc.insert (f x) n) HashMap.empty
+
+def mul (table: DBTable) (row: DBRow) : Nat :=
+  let value : Option Nat := table.get? row
+  match value with
+  | some n => n
+  | none => 0
+
+def insert (table: DBTable) (row: DBRow) (n : Nat) : DBTable :=
+  match table.mul row with
+  | 0 => HashMap.insert table row n
+  | m => HashMap.insert table row (m+n)
+
+def inter (t1 t2: DBTable) : DBTable :=
+  t1.fold
+    (fun acc x n1 =>
+     let n2 := DBTable.mul t2 x
+     let n := if n1 <= n2 then n1 else n2
+     if n > 0 then acc.insert x n else acc)
+    HashMap.empty
+
+def unionDisjoint (t1 t2: DBTable) : DBTable :=
+  t1.fold
+    (fun acc x n1 =>
+     let n2 := DBTable.mul t2 x
+     let n := n1 + n2
+     acc.insert x  n)
+    HashMap.empty
+
+def unionMax (t1 t2: DBTable) : DBTable :=
+  t1.fold
+    (fun acc x n1 =>
+     let n2 := DBTable.mul t2 x
+     let n := if n1 >= n2 then n1 else n2
+     acc.insert x  n)
+    HashMap.empty
+
+def differenceSubtract (t1 t2: DBTable) : DBTable :=
+  t1.fold
+    (fun acc x n1 =>
+     let n2 := DBTable.mul t2 x
+     let n := if n1 >= n2 then n1-n2 else n2 - n1
+     if n > 0 then acc.insert x  n else acc)
+    HashMap.empty
+
+def differenceRemove (t1 t2: DBTable) : DBTable :=
+  t1.fold
+    (fun acc x n1 =>
+     let n2 := DBTable.mul t2 x
+     if n2 > 0 then acc else acc.insert x  n1)
+    HashMap.empty
+
+def setof (t : DBTable) : DBTable :=
+  t.map (fun _ _ => 1)
+
+
+def getAnyRow (t: DBTable) : Option DBRow :=
+  t.fold (fun acc _ _ => acc) none
+
+end DBTable
+
+def List.toMap (lst : List (DBRow × Nat)) : DBTable :=
+  lst.foldl (λ acc (x,n) => acc.insert x n) HashMap.empty
+
+instance : ToString DBValue where
+  toString
+    | .boolValue (some v) => toString v
+    | .boolValue none => "none"
+    | .intValue (some v) => toString v
+    | .intValue none => "none"
+    | .stringValue (some v) => toString v
+    | .stringValue none => "none"
+
+instance : ToString DBRow where
+  toString lst := List.toString lst
+
+instance : ToString (DBTable) where
+  toString table := toString  (table.toList.map (fun (x,n) => s! "({x},{n})"))
+
+def DatabaseInstance := HashMap String DBTable
+
+instance : BEq (DBRow) where
+  beq l1 l2 := l1 == l2
+
+instance : Hashable DBValue where
+  hash
+    | .boolValue (some v) => hash v
+    | .boolValue none => 0
+    | .intValue (some v) => hash v
+    | .intValue none => 0
+    | .stringValue (some v) => hash v
+    | .stringValue none => 0
+
+instance : Hashable DBRow where
+  hash lst := lst.foldl (fun acc x => mixHash acc (hash x)) 0
+
+def row1: DBRow := [.boolValue false,.intValue (some 30),.stringValue "Mixed"]
+def row2:DBRow := [.boolValue true, .intValue (some 15),.stringValue "lower"]
+def row3:DBRow := [.boolValue true, .intValue (some 10),.stringValue "UPPER"]
+def as' : DBTable := [(row1,1), (row2,1), (row3,1)].toMap
+def bs' : DBTable := [(row2,1), (row3,1)].toMap
+
+#eval DBTable.differenceSubtract as' bs'
+
+def DBTable.product (xs : DBTable) (ys : DBTable) : DBTable :=
+  xs.fold
+    (fun acc1 x n1 =>
+     ys.fold
+       (fun acc2 y n2 =>
+        let n := n1 * n2
+        let row := List.append x y
+        acc2.insert row n)
+       acc1)
+    HashMap.empty
+
+
+
+def r1 : DBRow := [.intValue (some 100)]
+def r2 : DBRow := [.intValue (some 10)]
+def r3 : DBRow := [.intValue (some 15)]
+def t1 : DBTable := [(r1, 1), (r2, 3),(r3,1)].toMap
+def t2 : DBTable := [(r1, 1), (r2, 2),(r3,1)].toMap
+
+#eval DBTable.inter t1 t2
+#eval DBTable.differenceSubtract t1 t2
+#eval DBTable.product t1 t2
+
+
+#eval Substring.mk "123456789" (String.Pos.mk 0) (String.Pos.mk 4)
+
+def semanticsQueryOp (s : SQLSemantics) (op: QueryOp) (l r : DBTable) : DBTable :=
+match op with
+| .unionAll  =>
+  let result := l.unionDisjoint r
+  match s with
+  | .bag => result
+  | .set => result.setof
+| .union  => (l.unionDisjoint r).setof
+| .intersectAll  =>
+  let result := l.inter r
+  match s with
+  | .bag => result
+  | .set => result.setof
+| .intersect  => (l.inter r).setof
+| .except  => l.setof.differenceSubtract r
+| .exceptAll  =>
+  match s with
+  | .bag => l.differenceSubtract r
+  | .set => l.setof.differenceSubtract r
+
+instance : ToString BoolExpr where
+  toString expr :=
+    match expr with
+    | .column i => s!"column {i}"
+    | .null => "null"
+    | .literal v => s!"literal {v}"
+    -- | .exists q => s!"exists {q}"
+    -- | .case c t e => s!"case {c} {t} {e}"
+    | _ => "unknown"
+
+
+#eval [1,2,3].take 2
+
+mutual
+partial def semanticsBoolExpr (s : SQLSemantics) (d: DatabaseInstance) (expr: BoolExpr) : DBRow → Option Bool :=
+  fun x : DBRow =>
+  match expr with
+  | .column i => match x.get! i with
+    | .boolValue v => v
+    | _ => none
+  | .null => none
+  | .literal v => v
+  | .exists q => !(semantics s d q).isEmpty
+  | .case c t e =>
+    let (c',t', e'):= (semanticsBoolExpr s d c, semanticsBoolExpr s d t, semanticsBoolExpr s d e)
+    let isTrue := fun y : DBRow =>
+      let result := (c' y)
+      result.isSome && result.get!
+    let ite := if isTrue x then t' x else e' x
+    ite
+  | .boolEqual a b =>
+    let (a', b') :=  (semanticsBoolExpr s d a x, semanticsBoolExpr s d b x)
+    match a', b' with
+    | some x, some y => x == y
+    | _, _ => none
+  | .stringEqual a b =>
+    let (a', b') :=  (semanticsStringExpr s d a x, semanticsStringExpr s d b x)
+    match a', b' with
+    | some x, some y => x == y
+    | _, _ => none
+  | .intEqual a b =>
+    let (a', b') :=  (semanticsIntExpr s d a x, semanticsIntExpr s d b x)
+    match a', b' with
+    | some x, some y => x == y
+    | _, _ => none
+  |.and a b =>
+    let (a', b') :=  (semanticsBoolExpr s d a x, semanticsBoolExpr s d b x)
+    match a', b' with
+    | some x, some y => x && y
+    | some false, none => false
+    | none, some false => false
+    | _, _ => none
+  |.or a b =>
+    let (a', b') :=  (semanticsBoolExpr s d a x, semanticsBoolExpr s d b x)
+    match a', b' with
+    | some x, some y => x || y
+    | some true, none => true
+    | none, some true => true
+    | _, _ => none
+  |.not a =>
+    let a' := semanticsBoolExpr s d a x
+    match a' with
+    | some x => not x
+    | none => none
+  | .lsInt a b =>
+    let (a', b') := (semanticsIntExpr s d a x, semanticsIntExpr s d b x)
+    match a', b' with
+    | some x, some y => some (x < y)
+    | _, _ => none
+  | .leqInt a b =>
+    let (a', b') := (semanticsIntExpr s d a x, semanticsIntExpr s d b x)
+    match a', b' with
+    | some x, some y => some (x <= y)
+    | _, _ => none
+  | .gtInt a b =>
+    let (a', b') := (semanticsIntExpr s d a x, semanticsIntExpr s d b x)
+    match a', b' with
+    | some x, some y => some (x > y)
+    | _, _ => none
+  | .geqInt a b =>
+    let (a', b') := (semanticsIntExpr s d a x, semanticsIntExpr s d b x)
+    match a', b' with
+    | some x, some y => some (x >= y)
+    | _, _ => none
+  | .lsString a b =>
+    let (a', b') := (semanticsStringExpr s d a x, semanticsStringExpr s d b x)
+    match a', b' with
+    | some x, some y => some (x < y)
+    | _, _ => none
+  | .leqString a b =>
+    let (a', b') := (semanticsStringExpr s d a x, semanticsStringExpr s d b x)
+    match a', b' with
+    | some x, some y => some (x <= y)
+    | _, _ => none
+  | .gtString a b =>
+    let (a', b') := (semanticsStringExpr s d a x, semanticsStringExpr s d b x)
+    match a', b' with
+    | some x, some y => some (x > y)
+    | _, _ => none
+  | .geqString a b =>
+    let (a', b') := (semanticsStringExpr s d a x, semanticsStringExpr s d b x)
+    match a', b' with
+    | some x, some y => some (x >= y)
+    | _, _ => none
+  | .isNullBool a =>
+    let a' := semanticsBoolExpr s d a x
+    a' == none
+  | .isNotNullBool a =>
+    let a' := semanticsBoolExpr s d a x
+    a' != none
+  | .isNullString a =>
+    let a' := semanticsStringExpr s d a x
+    a' == none
+  | .isNotNullString a =>
+    let a' := semanticsStringExpr s d a x
+    a' != none
+  | .isNullInt a =>
+    let a' := semanticsIntExpr s d a x
+    a' == none
+  | .isNotNullInt a =>
+    let a' := semanticsIntExpr s d a x
+    a' != none
+  | .isTrue a =>
+    let a' := semanticsBoolExpr s d a x
+    a' == some true
+  | .isNotTrue a =>
+    let a' := semanticsBoolExpr s d a x
+    a' != some true
+
+
+partial def semanticsIntExpr (s : SQLSemantics) (d: DatabaseInstance) (expr: IntExpr) : DBRow → Option Int :=
+ fun x : DBRow =>
+ match expr with
+ | .column i => match x.get! i with
+    | .intValue v => v
+    | _ => none
+ | .null => none
+ | .literal v => v
+ | .plus a b =>
+    let (a', b') := (semanticsIntExpr s d a x, semanticsIntExpr s d b x)
+    match a', b' with
+    | none, _ => none
+    | _, none => none
+    | some c, some d => c + d
+ | .minus a b =>
+    let (a', b') := (semanticsIntExpr s d a x, semanticsIntExpr s d b x)
+    match a', b' with
+    | none, _ => none
+    | _, none => none
+    | some c, some d => c - d
+ | .multiplication a b =>
+    let (a', b') := (semanticsIntExpr s d a x, semanticsIntExpr s d b x)
+    match a', b' with
+    | none, _ => none
+    | _, none => none
+    | some c, some d => c * d
+ | .division a b =>
+    let (a', b') := (semanticsIntExpr s d a x, semanticsIntExpr s d b x)
+    match a', b' with
+    | none, _ => none
+    | _, none => none
+    | some c, some d => c / d
+ | .case c t e =>
+    let c' := semanticsBoolExpr s d c
+    let t' := semanticsIntExpr s d t
+    let e' := semanticsIntExpr s d e
+    let isTrue := fun y : DBRow =>
+      let result := (c' y)
+      result.isSome && result.get!
+    let ite := if isTrue x then t' x else e' x
+    ite
+
+partial def semanticsStringExpr (s : SQLSemantics) (d: DatabaseInstance) (expr: StringExpr) : DBRow → Option String :=
+ fun x : DBRow =>
+ match expr with
+ | .column i => match x.get! i with
+    | .stringValue v => v
+    | _ => none
+ | .null => none
+ | .literal v => v
+ | .upper a =>
+    match semanticsStringExpr s d a x with
+    | some str => str.toUpper
+    | none => none
+ | .lower a =>
+    match semanticsStringExpr s d a x with
+    | some str => str.toLower
+    | none => none
+ | .concat a b =>
+    let (a', b') := (semanticsStringExpr s d a x, semanticsStringExpr s d b x)
+    match a', b' with
+    | none, _ => none
+    | _, none => none
+    | some c, some d => c.append d
+ | .substring a start length =>
+    match semanticsStringExpr s d a x with
+    | some str => Substring.mk str (String.Pos.mk (start - 1)) (String.Pos.mk length) |>.toString
+    | _ => none
+ | .case c t e =>
+    let c' := semanticsBoolExpr s d c
+    let t' := semanticsStringExpr s d t
+    let e' := semanticsStringExpr s d e
+    let isTrue := fun y : DBRow =>
+      let result := (c' y)
+      result.isSome && result.get!
+    let ite := if isTrue x then t' x else e' x
+    ite
+
+partial def semanticsExpr (s : SQLSemantics) (d: DatabaseInstance) (e : Expr): DBRow → DBValue :=
+  fun x =>
+  match e with
+  |.boolExpr e' => .boolValue (semanticsBoolExpr s d e' x)
+  |.stringExpr e' => .stringValue (semanticsStringExpr s d e' x)
+  |.intExpr e' => .intValue (semanticsIntExpr s d e' x)
+
+
+
+partial def semantics (s : SQLSemantics) (d: DatabaseInstance) (q : Query) : DBTable :=
+  match q with
+  | .baseTable name =>
+    d.get! name
+  | .project exprs q =>
+   let q' := semantics s d q
+   let f := exprs.map (semanticsExpr s d)
+   let f' : DBRow → DBRow := fun x : DBRow => f.map (fun g => g x)
+   let q'' := q'.mapRow f'
+   q''
+  | .join l r join condition =>
+    let (l', r') := (semantics s d l, semantics s d r)
+    let product := DBTable.product l' r'
+    let p := semanticsBoolExpr s d condition
+    let result : DBTable := product.filter (fun x _ => (p x).isSome && (p x).get!)
+    if product.isEmpty then product
+    else
+    let leftLength := l'.getAnyRow.get!.length
+    let rightLength := r'.getAnyRow.get!.length
+    let nullsRow (t : DBRow) : DBRow :=
+      t.map (fun x => match x with
+          | .boolValue _ => .boolValue (none : Option Bool)
+          | .intValue _ => .intValue (none : Option Int)
+          | .stringValue _ => .stringValue (none : Option String)
+        )
+    match join with
+     | .inner => result
+     | .left =>
+      let minus := l'.differenceSubtract  (result.mapRow (fun x => x.take leftLength))
+      let nullsRight := nullsRow r'.getAnyRow.get!
+      let minusNulls := minus.mapRow (fun x => List.append x nullsRight)
+      result.unionDisjoint minusNulls
+     | .right =>
+      let minus := r'.differenceSubtract (result.mapRow (fun x => x.drop leftLength))
+      let nullsLeft := nullsRow l'.getAnyRow.get!
+      let minusNulls := minus.mapRow (fun x => List.append nullsLeft  x)
+      result.unionDisjoint minusNulls
+     | .full =>
+      let leftProject := result.mapRow (fun x => x.take leftLength)
+      let minus1 := l'.differenceSubtract leftProject
+      let nullsRight := nullsRow r'.getAnyRow.get!
+      let nulls1 := minus1.mapRow (fun x => List.append x nullsRight)
+      let rightProject := result.mapRow (fun x => x.drop leftLength)
+      let minus2 := r'.differenceSubtract rightProject
+      let nullsLeft := nullsRow l'.getAnyRow.get!
+      let nulls2 := minus2.mapRow (fun x => List.append nullsLeft x)
+      (result.unionDisjoint nulls1).unionDisjoint nulls2
+  | .filter condition q =>
+    let q' := semantics s d q
+    let p := semanticsBoolExpr s d condition
+    let q'' := q'.filter (fun x _ => (p x).isSome && (p x).get!)
+    q''
+  | .queryOperation op l r => semanticsQueryOp s op (semantics s d l) (semantics s d r)
+  | .values rows _ =>
+      rows.foldl
+      (fun acc row =>
+       let row' := row.map (fun e => match e with
+         | .boolExpr e' => .boolValue (semanticsBoolExpr s d e' [])
+         | .stringExpr e' => .stringValue (semanticsStringExpr s d e' [])
+         | .intExpr e' => .intValue (semanticsIntExpr s d e' []))
+       acc.insert row' 1)
+      HashMap.empty
+
+end
+
+
+def r1' : DBRow × Nat := ([.boolValue true, .intValue (some 10), .stringValue "UPPER"],1)
+def r2' : DBRow × Nat := ([.boolValue true, .intValue (some 15), .stringValue "lower"],1)
+def r3' : DBRow × Nat := ([.boolValue false, .intValue (some 08), .stringValue "Mixed"],1)
+def r4' : DBRow × Nat := ([.boolValue false, .intValue (some 30), .stringValue "Mixed"], 1)
+def table1 : DBTable := [r1', r2', r3'].toMap
+
+
+def table2 : DBTable := [r1', r2', r4'].toMap
+
+def d: DatabaseInstance := (HashMap.empty.insert "table1" table1).insert "table2" table2
+
+#eval d
+
+def q1: Query := .filter (BoolExpr.column 0) (.baseTable "table1")
+def q2: Query :=
+  let project := .project [.stringExpr (.upper (.column 2)), .intExpr (.multiplication (.column 1) (.literal 2))] (.baseTable "table")
+  let filter := .filter (.lsInt (.column 1) (.literal 25)) project
+  filter
+
+def q3 : Query := .join (.baseTable "table1") (.baseTable "table2") .full (.intEqual (.column 1) (.column 4))
+
+def q4 : Query := .values [[.boolExpr (.null), .intExpr (.null), .stringExpr (.null)]]
+                          [.sqlType .boolean true, .sqlType .integer true, .sqlType .text true ]
+
+#eval semantics .bag d q1
+#eval semantics .bag d q2
+#eval semantics .bag d q3
+#eval semantics .bag d q4
+
+
+def q:Query :=
+  .queryOperation .unionAll
+    (.queryOperation .exceptAll q1 q2)
+    (.queryOperation .exceptAll q1 q2)
